ArchSemArm/VMSA22Arm.v
@@ -656,15 +656,69 @@ Section VMSAArm.
       translation_internal : trfi ⊆ not_after cd;
       external : grel_irreflexive ob;
       atomic : (rmw ∩ (fre⨾ coe)) = ∅;
+      co_contains_TBLI_writes:
+      ∀ weid ∈ mem_writes cd, ∀ teid ∈ TLBI,
+        (weid, teid) ∈ coherence cd ∨ (teid, weid) ∈ coherence cd
+    }.
+  #[export] Instance consistent_dec : Decision consistent.
+  Proof.
+    destruct decide (exp_internal cd).
+    2: right; abstract (by intros []).
+    destruct decide (reg_internal cd).
+    2: right; abstract (by intros []).
+    destruct decide (trfi ⊆ not_after cd).
+    2: right; abstract (by intros []).
+    destruct decide (grel_irreflexive ob).
+    2: right; abstract (by intros []).
+    destruct decide ((rmw ∩ (fre⨾ coe)) = ∅).
+    2: right; abstract (by intros []).
+    destruct decide (
+        ∀ weid ∈ mem_writes cd, ∀ teid ∈ TLBI,
+          (weid, teid) ∈ coherence cd ∨ (teid, weid) ∈ coherence cd).
+    2: right; abstract (by intros []).
+    left. abstract done.
+  Defined.
+
+  Record not_UB := {
       initial_reads : IF ⊆ IR;
       initial_reads_not_delayed : IF ## grel_rng (coherence cd);
       register_write_permitted : Illegal_RW = ∅;
       memory_events_permitted : (mem_events cd) ⊆ M ∪ T ∪ IF;
       is_nms' : is_nms cd;
       no_cacheop : ICDC = ∅;
-      co_contains_TBLI_writes:
-      ∀ weid ∈ mem_writes cd, ∀ teid ∈ TLBI,
-        (weid, teid) ∈ coherence cd ∨ (teid, weid) ∈ coherence cd
     }.
+  #[export] Instance not_UB_dec : Decision not_UB.
+  Proof.
+    destruct decide (IF ⊆ IR).
+    2: right; abstract (by intros []).
+    destruct decide (IF ## grel_rng (coherence cd)).
+    2: right; abstract (by intros []).
+    destruct decide (Illegal_RW = ∅).
+    2: right; abstract (by intros []).
+    destruct decide ((mem_events cd) ⊆ M ∪ T ∪ IF).
+    2: right; abstract (by intros []).
+    destruct decide (is_nms cd).
+    2: right; abstract (by intros []).
+    destruct decide (ICDC = ∅).
+    2: right; abstract (by intros []).
+    left. abstract done.
+  Defined.
+
+  Definition consistent_ok := consistent ∧ not_UB.
+  Instance consistent_ok_dec : Decision consistent_ok.
+  Proof. unfold_decide. Defined.
 
 End VMSAArm.
+
+Require Import ASCommon.CResult.
+
+(** The SC Arm axiomatic model *)
+Definition axmodel regs_whitelist : Ax.t NMS ∅ :=
+  λ _ cd, if decide (consistent cd) then
+            if decide (not_UB regs_whitelist cd) then Ok Ax.Allowed
+            else Error ""
+          else Ok Ax.Rejected.
+
+(** The SC Arm architecture model *)
+Definition archmodel regs_whitelist isem : Model.nc ∅ :=
+  Ax.to_Modelnc isem (axmodel regs_whitelist).
