ArchSem/CandidateExecutions.v
@@ -531,6 +531,9 @@ Module CandidateExecutions (IWA : InterfaceWithArch) (Term : TermModelsT IWA) (N
 
       Definition has_only_supported_events pe : Prop :=
         iEvent_list pe |> filter (λ '(_,ev), unsupported_event ev) = [].
+      #[export] Instance has_only_supported_events_dec cd :
+        Decision (has_only_supported_events cd).
+      Proof. unfold has_only_supported_events. tc_solve. Defined.
 
       (** * Final register map *)
       (** Get the final register maps of all threads from a pre-execution. If
@@ -858,6 +861,8 @@ Module CandidateExecutions (IWA : InterfaceWithArch) (Term : TermModelsT IWA) (N
 
       (** Decide if a pre-execution does not involve mixed size accesses *)
       Definition is_nms pe := overlapping pe ⊆ same_footprint pe.
+      #[export] Instance is_nms_dec pe : Decision (is_nms pe).
+      Proof. unfold is_nms. tc_solve. Defined.
 
       (** ** Register based relations *)
 
@@ -932,7 +937,9 @@ Module CandidateExecutions (IWA : InterfaceWithArch) (Term : TermModelsT IWA) (N
         guard' (
             mem_lookup addr (bvn_n val / 8) pe.(init).(MState.memory)
               |$> bv_to_bvn = Some val).
-
+      #[export] Instance is_valid_init_mem_read_dec pe eid :
+        Decision (is_valid_init_mem_read pe eid).
+      Proof. unfold is_valid_init_mem_read. tc_solve. Defined.
 
       (** ** Not after
 
@@ -1143,7 +1150,9 @@ Module CandidateExecutions (IWA : InterfaceWithArch) (Term : TermModelsT IWA) (N
              that both accesses are the same size *)
       end.
 
-
+    Instance is_valid_rf_dec {cd : t} weid reid :
+      Decision (is_valid_rf cd weid reid).
+    Proof. unfold is_valid_rf. tc_solve. Defined.
 
     Record reads_from_wf {cd : t} :=
       {
@@ -1156,6 +1165,20 @@ Module CandidateExecutions (IWA : InterfaceWithArch) (Term : TermModelsT IWA) (N
       }.
     #[global] Arguments reads_from_wf : clear implicits.
 
+    Instance reads_from_wf_dec {cd : t} : Decision (reads_from_wf cd).
+    Proof.
+      destruct decide (grel_dom (reads_from cd) ⊆ (mem_writes cd)).
+      2: right; abstract (by intros []).
+      destruct decide (grel_rng (reads_from cd) ⊆ (mem_reads cd)).
+      2: right; abstract (by intros []).
+      destruct decide (grel_functional (reads_from cd)⁻¹).
+      2: right; abstract (by intros []).
+      destruct decide (∀'(weid, reid) ∈ reads_from cd, is_valid_rf cd weid reid).
+      2: right; abstract (by intros []).
+      destruct decide (∀ reid ∈ init_mem_reads cd, is_valid_init_mem_read cd reid).
+      2: right; abstract (by intros []).
+      left. abstract done.
+    Defined.
 
     (** *** Coherence wellformedness *)
 
@@ -1170,6 +1193,20 @@ Module CandidateExecutions (IWA : InterfaceWithArch) (Term : TermModelsT IWA) (N
           (weid1, weid2) ∈ coherence cd ∨ (weid2, weid1) ∈ coherence cd
       }.
     #[global] Arguments coherence_wf : clear implicits.
+    Instance coherence_wf_dec {cd : t} : Decision (coherence_wf cd).
+    Proof.
+      destruct decide (grel_transitive (coherence cd)).
+      2: right; abstract (by intros []).
+      destruct decide (grel_irreflexive (coherence cd)).
+      2: right; abstract (by intros []).
+      destruct decide
+        (∀ weid1 weid2 ∈ mem_writes cd,
+           is_overlapping cd weid1 weid2 →
+           (weid1, weid2) ∈ coherence cd ∨ (weid2, weid1) ∈ coherence cd).
+      2: right; abstract (by intros []).
+      left. abstract done.
+    Defined.
+
 
     (** *** lxsx wellformedness *)
 
@@ -1181,6 +1218,18 @@ Module CandidateExecutions (IWA : InterfaceWithArch) (Term : TermModelsT IWA) (N
         lxsx_same_pa : lxsx cd ⊆ same_addr cd
       }.
     #[global] Arguments lxsx_wf : clear implicits.
+    Instance lxsx_wf_dec {cd : t} : Decision (lxsx_wf cd).
+    Proof.
+      destruct decide (grel_dom (lxsx cd) ⊆ exclusive_reads cd).
+      2: right; abstract (by intros []).
+      destruct decide (grel_rng (lxsx cd) ⊆ exclusive_writes cd).
+      2: right; abstract (by intros []).
+      destruct decide (lxsx cd ⊆ instruction_order cd).
+      2: right; abstract (by intros []).
+      destruct decide (lxsx cd ⊆ same_addr cd).
+      2: right; abstract (by intros []).
+      left. abstract done.
+    Defined.
 
 
     (** *** Reg reads from wellformedness
@@ -1199,6 +1248,20 @@ Module CandidateExecutions (IWA : InterfaceWithArch) (Term : TermModelsT IWA) (N
           initial_reg_reads cd ⊆ possible_initial_reg_reads cd;
       }.
     #[global] Arguments reg_reads_from_wf : clear implicits.
+    Instance reg_reads_from_wf_dec {cd : t} : Decision (reg_reads_from_wf cd).
+    Proof.
+      destruct decide (grel_dom (reg_reads_from cd) ⊆ (reg_writes cd)).
+      2: right; abstract (by intros []).
+      destruct decide (grel_rng (reg_reads_from cd) ⊆ (reg_reads cd)).
+      2: right; abstract (by intros []).
+      destruct decide (grel_functional (reg_reads_from cd)⁻¹).
+      2: right; abstract (by intros []).
+      destruct decide (reg_reads_from cd ⊆ same_reg_val cd).
+      2: right; abstract (by intros []).
+      destruct decide (initial_reg_reads cd ⊆ possible_initial_reg_reads cd).
+      2: right; abstract (by intros []).
+      left. abstract done.
+    Defined.
 
     Lemma rrf_irreflexive (cd : t) :
       reg_reads_from_wf cd → grel_irreflexive (reg_reads_from cd).
@@ -1234,6 +1297,10 @@ Module CandidateExecutions (IWA : InterfaceWithArch) (Term : TermModelsT IWA) (N
         if get_addr_space ev is Some a
         then a = cd.(init).(MState.address_space)
         else True.
+    Instance addr_space_wf_dec {cd : t} : Decision (addr_space_wf cd).
+    Proof. unfold addr_space_wf. tc_solve. Defined.
+
+
 
     Record footprint_wf {cd : t} :=
       {
@@ -1255,6 +1322,27 @@ Module CandidateExecutions (IWA : InterfaceWithArch) (Term : TermModelsT IWA) (N
           else True
       }.
     #[global] Arguments footprint_wf : clear implicits.
+    Instance footprint_wf_dec {cd : t} : Decision (footprint_wf cd).
+    Proof.
+      destruct decide (
+          ∀ tid : fin nmth,
+            ∀ instr ∈ cd.(events) !!! tid,
+            ∀ ev ∈ fst instr,
+            if get_reg ev is Some reg
+            then reg ∈ dom (cd.(init).(MState.regs) !!! tid)
+            else True).
+      2: right; abstract (by intros []).
+      destruct decide (
+          ∀ '(eid, ev) ∈ event_list cd,
+            if get_addr ev is Some addr then
+              if get_size ev is Some n then
+                ∀ addr' ∈ addr_range addr n, addr' ∈ dom cd.(init).(MState.memory)
+          else False
+          else True).
+      2: right; abstract (by intros []).
+      left. abstract done.
+    Defined.
+
 
     Record wf (cd : t) :=
       {
@@ -1266,7 +1354,26 @@ Module CandidateExecutions (IWA : InterfaceWithArch) (Term : TermModelsT IWA) (N
         lxsx_wf' :> lxsx_wf cd;
         reg_reads_from_wf' :> reg_reads_from_wf cd;
       }.
+    Instance wf_dec cd : Decision (wf cd).
+    Proof.
+      destruct decide (has_only_supported_events cd).
+      2: right; abstract (by intros []).
+      destruct decide (addr_space_wf cd).
+      2: right; abstract (by intros []).
+      destruct decide (footprint_wf cd).
+      2: right; abstract (by intros []).
+      destruct decide (reads_from_wf cd).
+      2: right; abstract (by intros []).
+      destruct decide (coherence_wf cd).
+      2: right; abstract (by intros []).
+      destruct decide (lxsx_wf cd).
+      2: right; abstract (by intros []).
+      destruct decide (reg_reads_from_wf cd).
+      2: right; abstract (by intros []).
+      left. abstract done.
+    Defined.
     End Cand.
+
 
     (** * Dependency relations *)
 
